Veritas.Verifier.Merkle.fsti
@@ -1,6 +1,7 @@
 module Veritas.Verifier.Merkle
 
 open Veritas.BinTree
+open Veritas.Hash
 open Veritas.Key
 open Veritas.Record
 open Veritas.Verifier.CorrectDefs
@@ -14,8 +15,17 @@ let mv_points_to_some (v:merkle_value) (d:bin_tree_dir): bool =
 let mv_pointed_key (v:merkle_value) (d:bin_tree_dir{mv_points_to_some v d}): key = 
   Desc?.k (desc_hash_dir v d)
 
+let mv_pointed_hash (v:merkle_value) (d:bin_tree_dir{mv_points_to_some v d}): hash_value = 
+  Desc?.h (desc_hash_dir v d)
+
 let mv_points_to (v:merkle_value) (d:bin_tree_dir) (k:key): bool = 
   mv_points_to_some v d && mv_pointed_key v d = k
+
+let mv_evicted_to_blum (v:merkle_value) (d:bin_tree_dir {mv_points_to_some v d}): bool =
+  Desc?.b (desc_hash_dir v d)
+
+let eac_merkle_value (#p:pos) (itsl: eac_ts_log p) (k:merkle_key): merkle_value =
+  to_merkle_value (eac_value itsl k)
 
 (* the ancestor who holds the proof of the value of key k *)
 val proving_ancestor (#p:pos) (itsl: eac_ts_log p) (k:key{k <> Root}):
@@ -24,14 +34,30 @@ val proving_ancestor (#p:pos) (itsl: eac_ts_log p) (k:key{k <> Root}):
 (* after the first add the proving ancestor always points to self *)
 val lemma_proving_ancestor_points_to_self (#p:pos) (itsl: eac_ts_log p) (k:key{k <> Root}):
   Lemma (requires not (is_eac_state_init itsl k))
-        (ensures (mv_points_to (to_merkle_value (eac_value itsl (proving_ancestor itsl k)))
+        (ensures (mv_points_to (eac_merkle_value itsl (proving_ancestor itsl k))
                                (desc_dir k (proving_ancestor itsl k))
                                k))
+        [SMTPat (proving_ancestor itsl k)]
 
 (* before the first add the proving ancestor points to none or to a key that is not an ancestor *)
 val lemma_proving_ancestor_initial (#p:pos) (itsl: eac_ts_log p) (k:key{k <> Root}):
   Lemma (requires (is_eac_state_init itsl k))
-        (ensures (mv_points_to_none (to_merkle_value (eac_value itsl (proving_ancestor itsl k)))
+        (ensures (mv_points_to_none (eac_merkle_value itsl (proving_ancestor itsl k))
                                     (desc_dir k (proving_ancestor itsl k)) \/
-                  not (is_desc k (mv_pointed_key (to_merkle_value (eac_value itsl (proving_ancestor itsl k)))
+                  not (is_desc k (mv_pointed_key (eac_merkle_value itsl (proving_ancestor itsl k))
                                                  (desc_dir k (proving_ancestor itsl k))))))
+
+(* when evicted as merkle the proving ancestor contains our hash *)
+val lemma_proving_ancestor_has_hash (#p:pos) (itsl: eac_ts_log p) (k:key{k<> Root}):
+  Lemma (requires (is_eac_state_evicted_merkle itsl k))
+        (ensures (mv_pointed_hash (eac_merkle_value itsl (proving_ancestor itsl k))
+                                  (desc_dir k (proving_ancestor itsl k)) = 
+                  hashfn (eac_value itsl k)))
+
+(* when evicted as blum the proving ancestor contains a bit indicating the eviction *)
+val lemma_proving_ancestor_blum_bit (#p:pos) (itsl: eac_ts_log p) (k:key{k <> Root}):
+  Lemma (requires (is_eac_state_evicted itsl k))
+        (ensures (mv_evicted_to_blum (eac_merkle_value itsl (proving_ancestor itsl k))
+                                     (desc_dir k (proving_ancestor itsl k)) = 
+                  is_eac_state_evicted_blum itsl k))
+      
